refactor ibackend slightly
- use inc_config instead of mconfig

compiler/backend/icompile/ibackendScript.sml
@@ -3,7 +3,7 @@
   meant to be syntactically equal to backend but allows
   compiling program in a part-by-part manner
 *)
-open preamble backendTheory namespacePropsTheory;
+open preamble backend_asmTheory namespacePropsTheory;
 
 val _ = new_theory"ibackend";
 
@@ -20,18 +20,18 @@ val _ = new_theory"ibackend";
 
   2. icompile:
 
-    This should run incremental compilation on a chunk of
-    input source program.
+    This should run incremental compilation on separate
+    chunks of an incrementally defined input source program.
 
   3. end_icompile:
 
     This should "end" compilation by inserting the main
-    entry point of the whole program.
+    entry point of the whole program and cleaning up.
 
-  Then, we'll do a whole program assembly step
+  The above steps will get us to labLang.
 
-  4. assemble/finalize
-
+  Then, we'll do a whole program assembly step to get the
+  final program.
 *)
 
 (******************************************************************************)
@@ -44,7 +44,8 @@ val _ = new_theory"ibackend";
   TODO: the _alt parts of this definition will eventually need to be proved
   and moved into backend/ *)
 
-(* NOTE: change the order of chain_exps *)
+(* NOTE: change the order of prog going into clos_annotate
+  clos_to_bvlTheory.compile_common_def *)
 Definition clos_to_bvl_compile_common_alt_def:
   clos_to_bvl_compile_common_alt c es =
     let es = clos_mti$compile c.do_mti c.max_app es in
@@ -57,11 +58,14 @@ Definition clos_to_bvl_compile_common_alt_def:
     let aux = REVERSE aux in
     let prog = aux ++ (chain_exps n es) in
     let prog = clos_annotate$compile prog in
-      (c with <| start := n; next_loc := n + MAX 1 (LENGTH es); known_conf := kc;
-                 call_state := (g,aux) |>,
+      (c with <| start := n; next_loc := n + MAX 1 (LENGTH es);
+        known_conf := kc; call_state := (g,aux) |>,
        prog)
 End
 
+(* A new "top" function that keeps a compiled exp and
+  its auxliaries (aux) close by.
+  clos_to_bvlTheory.compile_prog_def *)
 Definition clos_to_bvl_compile_prog_top_def:
   clos_to_bvl_compile_prog_top max_app (prog: (num # num # closLang$exp) list) =
   MAP (\(loc, args, e).
@@ -70,6 +74,8 @@ Definition clos_to_bvl_compile_prog_top_def:
       ) prog
 End
 
+(* Replaces compile_common and compile_prog.
+  clos_to_bvlTheory.compile_def *)
 Definition clos_to_bvl_compile_alt_def:
   clos_to_bvl_compile_alt c0 es =
     let (c, prog) = clos_to_bvl_compile_common_alt c0 es in
@@ -82,6 +88,7 @@ Definition clos_to_bvl_compile_alt_def:
       (c, prog')
 End
 
+(* bvl_to_bviTheory.stubs_def *)
 Definition bvi_stubs_without_init_globs_def:
   bvi_stubs_without_init_globs =
   [(AllocGlobal_location, AllocGlobal_code);
@@ -93,6 +100,7 @@ Definition bvi_stubs_without_init_globs_def:
    (ConcatByte_location, ConcatByte_code)]
 End
 
+(* bvl_to_bviTheory.compile_prog_def *)
 Definition bvl_to_bvi_compile_prog_alt_def:
   bvl_to_bvi_compile_prog_alt start n prog =
     let k = alloc_glob_count (MAP (\(_,_,p). p) prog) in
@@ -102,7 +110,8 @@ Definition bvl_to_bvi_compile_prog_alt_def:
       (InitGlobals_location, bvi_stubs_without_init_globs ++ append code ++ init_globs_stub, n1)
 End
 
-(* change the order of the stubs *)
+(* change the order of the stubs
+  bvl_to_bviTheory.compile_def *)
 Definition bvl_to_bvi_compile_alt_def:
   bvl_to_bvi_compile_alt start (c: bvl_to_bvi$config) names prog =
     let (inlines, prog) = bvl_inline$compile_prog c.inline_size_limit
@@ -112,7 +121,7 @@ Definition bvl_to_bvi_compile_alt_def:
       (loc, code', inlines, n1, n2, get_names (MAP FST code') names)
 End
 
-(* collate all the things *)
+(* collate all the config updates *)
 Definition bvl_to_bvi_compile_update_config_def:
   bvl_to_bvi_compile_update_config clos_conf bvl_conf p =
   let (s, p, l, n1, n2, _) =
@@ -122,39 +131,14 @@ Definition bvl_to_bvi_compile_update_config_def:
     (clos_conf, bvl_conf, p)
 End
 
-(* no raw call TODO: use new rawcall config *)
-Definition stack_to_lab_compile_alt_def:
-  stack_to_lab_compile_alt stack_conf data_conf max_heap sp offset prog =
-  let prog = stack_alloc$compile data_conf prog in
-  let prog = stack_remove$compile stack_conf.jump offset (is_gen_gc data_conf.gc_kind)
-                                  max_heap sp InitGlobals_location prog in
-  let prog = stack_names$compile stack_conf.reg_names prog in
-     MAP prog_to_section prog
-End
-
-
-
-Datatype:
-  mconfig =
-  <| source_conf : source_to_flat$config;
-     clos_conf : clos_to_bvl$config;
-     bvl_conf : bvl_to_bvi$config;
-     data_conf : data_to_word$config;
-     word_to_word_conf: word_to_word$config;
-     word_to_stack_conf : word_to_stack$config;
-     stack_conf: stack_to_lab$config;
-  |>
-End
-
-
-Definition compile_alt1_def:
-  compile_alt1 (asm_conf: 'a asm_config) (c : mconfig) p =
-  let source_conf = c.source_conf in
-  let clos_conf = c.clos_conf in
-  let bvl_conf = c.bvl_conf in
-  let data_conf = c.data_conf in
-  let word_to_word_conf = c.word_to_word_conf in
-  let stack_conf = c.stack_conf in
+Definition compile_alt_def:
+  compile_alt (asm_conf: 'a asm_config) (c : inc_config) p =
+  let source_conf = c.inc_source_conf in
+  let clos_conf = c.inc_clos_conf in
+  let bvl_conf = c.inc_bvl_conf in
+  let data_conf = c.inc_data_conf in
+  let word_to_word_conf = c.inc_word_to_word_conf in
+  let stack_conf = c.inc_stack_conf in
   let p = source_to_source$compile p in
   let (source_conf', compiled_p_flat) =
     source_to_flat$compile source_conf p in
@@ -173,47 +157,17 @@ Definition compile_alt1_def:
   let max_heap = (2 * data_to_word$max_heap_limit (:'a) data_conf - 1) in
   let sp = (asm_conf.reg_count - (LENGTH asm_conf.avoid_regs + 3)) in
   let offset = asm_conf.addr_offset in
-  let (stack_conf', compiled_p_lab) = stack_to_lab$compile stack_conf data_conf max_heap sp offset compiled_p_stack in
+  let compiled_p_lab = stack_to_lab$compile stack_conf data_conf max_heap sp offset compiled_p_stack in
   let c' = c with
-             <| source_conf := source_conf';
-                clos_conf := clos_conf';
-                bvl_conf := bvl_conf';
-                word_to_stack_conf := word_to_stack_conf;
-                stack_conf := stack_conf'
+             <| inc_source_conf := source_conf';
+                inc_clos_conf := clos_conf';
+                inc_bvl_conf := bvl_conf';
+                inc_word_conf := word_to_stack_conf
              |> in
     (c', bm, compiled_p_lab)
 End
 
-Definition to_livesets_0_alt_def:
-  to_livesets_0_alt asm_conf (word_conf, p) =
-  let alg = word_conf.reg_alg in
-  let p = word_internal asm_conf p in
-  let data = MAP (\(name_num,arg_count,prog).
-  let (heu_moves,spillcosts) = get_heuristics alg name_num prog in
-  (get_clash_tree prog,heu_moves,spillcosts,
-    get_forced asm_conf prog [],get_stack_only prog)) p
-  in
-    ((asm_conf.reg_count - (5+LENGTH asm_conf.avoid_regs),data), p)
-End
-
-Definition to_livesets_alt_def:
-  to_livesets_alt source_conf clos_conf bvl_conf data_conf word_conf asm_conf p =
-  let p = source_to_source$compile p in
-  let (source_conf', compiled_p_flat) =
-    source_to_flat$compile source_conf p in
-  let compiled_p_clos =
-    flat_to_clos$compile_prog compiled_p_flat in
-  let (clos_conf', compiled_p_bvl) =
-    clos_to_bvl_compile_alt clos_conf compiled_p_clos in
-  let (clos_conf', bvl_conf', compiled_p_bvi) =
-    bvl_to_bvi_compile_update_config clos_conf' bvl_conf compiled_p_bvl in
-  let compiled_p_data =
-    bvi_to_data$compile_prog compiled_p_bvi in
-  let compiled_p_word_0 = data_to_word$compile_0 data_conf asm_conf compiled_p_data in
-  let ((reg_count, data), p) = to_livesets_0_alt asm_conf (word_conf, compiled_p_word_0) in
-    (source_conf', clos_conf', bvl_conf', (reg_count, data), p)
-End
-
+(* Configurations for incremental compilation *)
 Datatype:
   source_iconfig =
   <| n : num ;
@@ -253,12 +207,13 @@ Datatype:
 End
 
 Datatype:
-  word_to_stack_iconfig = <| k : num ;
-                             bm : 'a word app_list # num ;
-                             sfs_list : (num # num) list;
-                             fs : num list
-                          |>
+  word_iconfig = <| k : num ;
+                    bm : 'a word app_list # num ;
+                    sfs_list : (num # num) list;
+                    fs : num list
+                  |>
 End
+
 (*
 Definition empty_word_to_stack_iconf_def:
     empty_word_to_stack_iconf = (<| k := 0n;
@@ -273,12 +228,13 @@ Datatype:
   <| source_iconf : source_iconfig;
      clos_iconf: clos_iconfig;
      bvl_iconf: bvl_iconfig;
-     data_conf: data_to_word$config;
-     word_to_word_conf: word_to_word$config;
-     word_to_stack_iconf: 'a word_to_stack_iconfig;
-     stack_conf: stack_to_lab$config;
+     data_conf : data_to_word$config;
+     word_to_word_conf : word_to_word$config;
+     word_iconf: 'a word_iconfig;
+     stack_conf : stack_to_lab$config
   |>
 End
+
 (*
 Datatype:
   iconfig_lvs =
@@ -291,6 +247,7 @@ Datatype:
 End
 *)
 
+(* source_to_flat *)
 Definition icompile_source_to_flat_def:
   icompile_source_to_flat source_iconf p =
   let n = source_iconf.n in
@@ -348,10 +305,9 @@ Definition end_icompile_source_to_flat_def:
                    mod_env := source_iconf.env |>
 End
 
-
+(* flat_to_clos *)
 Definition icompile_flat_to_clos_def:
-  icompile_flat_to_clos p =
-  flat_to_clos$compile_decs p
+  icompile_flat_to_clos p = flat_to_clos$compile_decs p
 End
 
 Definition init_icompile_flat_to_clos_def:
@@ -360,6 +316,7 @@ Definition init_icompile_flat_to_clos_def:
   clos_stub
 End
 
+(* clos_to_bvl *)
 Definition icompile_clos_to_bvl_common_def:
   icompile_clos_to_bvl_common (clos_iconf: clos_iconfig) p =
   let p = clos_mti$compile clos_iconf.do_mti clos_iconf.max_app p in
@@ -391,7 +348,6 @@ Definition icompile_clos_to_bvl_common_def:
   (clos_iconf, p)
 End
 
-(* TODO: modify this and try the rest *)
 Definition icompile_clos_to_bvl_prog_def:
   icompile_clos_to_bvl_prog max_app config_aux p  =
   let prog = MAP (SND o SND) p in
@@ -401,7 +357,6 @@ Definition icompile_clos_to_bvl_prog_def:
     (new_config_aux, new_bvl_exps)
 End
 
-
 Definition icompile_clos_to_bvl_def:
   icompile_clos_to_bvl (clos_iconf: clos_iconfig)  p =
   let (clos_iconf, p) = icompile_clos_to_bvl_common clos_iconf p in
@@ -409,7 +364,6 @@ Definition icompile_clos_to_bvl_def:
   let clos_iconf = clos_iconf with compile_exps_aux := aux in
     (clos_iconf, p)
 End
-
 
 Definition icompile_clos_to_bvl_alt_def:
   icompile_clos_to_bvl_alt (clos_iconf: clos_iconfig) p =
@@ -433,7 +387,6 @@ Definition init_icompile_clos_to_bvl_def:
                       compile_exps_aux := []|> in
   let init_stubs = toAList (init_code clos_iconf.max_app) in
   let (clos_iconf, bvl_stub) = icompile_clos_to_bvl_alt clos_iconf clos_stub in
-
     (clos_iconf, init_stubs ++ bvl_stub)
 End
 
@@ -454,15 +407,13 @@ Definition end_icompile_clos_to_bvl_def:
   (clos_conf, es_chained  ++ init_globs)
 End
 
-
-
-
+(* bvl_to_bvi *)
 Definition icompile_bvl_to_bvi_inline_def:
   icompile_bvl_to_bvi_inline limit split_seq cut_size cs p =
   bvl_inline$compile_inc limit split_seq cut_size cs p
 End
 
-(* will this result in inefficiencies due to the append code*)
+(* TODO: will this result in inefficiencies due to the append code *)
 Definition icompile_bvl_to_bvi_prog_def:
   icompile_bvl_to_bvi_prog n p k_acc =
   let k = bvl_to_bvi$alloc_glob_count (MAP (\(_,_,p). p) p) in
@@ -497,8 +448,6 @@ Definition init_icompile_bvl_to_bvi_def:
   let (bvl_iconf, bvi_stubs1) = icompile_bvl_to_bvi bvl_iconf bvl_init in
   (bvl_iconf,  bvi_stubs ++ bvi_stubs1)
 End
-
-
 
 Definition end_icompile_bvl_to_bvi_def:
   end_icompile_bvl_to_bvi bvl_end bvl_iconf clos_conf bvl_conf =
@@ -565,15 +514,13 @@ Definition end_icompile_word_to_stack_def:
           stack_frame_size := sfs |>, word_iconf.fs, stack_end)
 End
 
-(* we just carry on with the stack_conf, since its incremental anyways*)
+(* drop rawcall *)
 Definition icompile_stack_to_lab_def:
   icompile_stack_to_lab stack_conf offset k p =
-  let (i, p) = stack_rawcall$compile_aux stack_conf.rawcall_info p in
   let p = MAP stack_alloc$prog_comp p in
   let p = MAP (stack_remove$prog_comp stack_conf.jump offset k) p in
   let p = MAP (stack_names$prog_comp stack_conf.reg_names) p in
-  let c = stack_conf with rawcall_info := i in
-    (c, MAP stack_to_lab$prog_to_section p)
+    MAP stack_to_lab$prog_to_section p
 End
 
 Definition init_icompile_stack_to_lab_def:
@@ -583,18 +530,18 @@ Definition init_icompile_stack_to_lab_def:
                                    max_heap sp bvl_to_bvi$InitGlobals_location stubs in
   let stubs = stack_names$compile stack_conf.reg_names stubs in
   let stubs = MAP stack_to_lab$prog_to_section stubs in
-  let (stack_conf', p) = icompile_stack_to_lab stack_conf offset sp stack_init in
-    (stack_conf', stubs ++ p)
+  let p = icompile_stack_to_lab stack_conf offset sp stack_init in
+    stubs ++ p
 End
 
 Definition init_icompile_def:
-  init_icompile (asm_conf: 'a asm_config) (c: mconfig) =
-  let source_conf = c.source_conf in
-  let clos_conf = c.clos_conf in
-  let bvl_conf = c.bvl_conf in
-  let data_conf = c.data_conf in
-  let word_to_word_conf = c.word_to_word_conf in
-  let stack_conf = c.stack_conf in
+  init_icompile (asm_conf: 'a asm_config) (c: inc_config) =
+  let source_conf = c.inc_source_conf in
+  let clos_conf = c.inc_clos_conf in
+  let bvl_conf = c.inc_bvl_conf in
+  let data_conf = c.inc_data_conf in
+  let word_to_word_conf = c.inc_word_to_word_conf in
+  let stack_conf = c.inc_stack_conf in
   let (source_iconf, flat_stub) = init_icompile_source_to_flat source_conf in
   let clos_stub = init_icompile_flat_to_clos flat_stub in
   let (clos_iconf, bvl_init) = init_icompile_clos_to_bvl clos_conf clos_stub in
@@ -602,9 +549,9 @@ Definition init_icompile_def:
   let data_init = bvi_to_data$compile_prog bvi_init in
   let (data_conf', word_init) = init_icompile_data_to_word data_conf asm_conf data_init in
   let (_, word_init1) = word_to_word$compile word_to_word_conf asm_conf word_init in
-  let (word_to_stack_iconf, stack_init) = init_icompile_word_to_stack asm_conf word_init1 in
+  let (word_iconf, stack_init) = init_icompile_word_to_stack asm_conf word_init1 in
   let max_heap = (2 * data_to_word$max_heap_limit (:'a) data_conf - 1) in
-  let (stack_conf, lab_init) = init_icompile_stack_to_lab stack_conf data_conf
+  let lab_init = init_icompile_stack_to_lab stack_conf data_conf
                                             max_heap
                                             (asm_conf.reg_count - (LENGTH asm_conf.avoid_regs + 3))
                                             asm_conf.addr_offset stack_init in
@@ -613,26 +560,26 @@ Definition init_icompile_def:
               bvl_iconf := bvl_iconf;
               data_conf := data_conf';
               word_to_word_conf := word_to_word_conf;
-              word_to_stack_iconf := word_to_stack_iconf;
-              stack_conf := stack_conf;
+              word_iconf := word_iconf;
+              stack_conf := stack_conf
            |>
   in
     (ic, lab_init)
 End
 
 Definition end_icompile_def:
-  end_icompile asm_conf ic (c : mconfig)
+  end_icompile asm_conf (ic: 'a iconfig) (c : inc_config)
   =
   let source_iconf = ic.source_iconf in
   let clos_iconf = ic.clos_iconf in
   let bvl_iconf = ic.bvl_iconf in
   let data_conf = ic.data_conf in
-  let word_to_word_conf = ic.word_to_word_conf in
-  let word_to_stack_iconf = ic.word_to_stack_iconf in
-  let stack_conf = ic.stack_conf in
-  let source_conf = c.source_conf in
-  let clos_conf = c.clos_conf in
-  let bvl_conf = c.bvl_conf in
+  let word_to_word_conf = c.inc_word_to_word_conf in
+  let word_iconf = ic.word_iconf in
+  let stack_conf = c.inc_stack_conf in
+  let source_conf = c.inc_source_conf in
+  let clos_conf = c.inc_clos_conf in
+  let bvl_conf = c.inc_bvl_conf in
   let source_conf_after_ic = end_icompile_source_to_flat source_iconf source_conf in
   let (clos_conf_after_ic, bvl_end) = end_icompile_clos_to_bvl clos_iconf clos_conf in
   let (clos_conf_after_ic_bvi, bvl_conf_after_ic, bvi_end) =
@@ -640,27 +587,26 @@ Definition end_icompile_def:
   let data_end = bvi_to_data$compile_prog bvi_end in
   let word_end = icompile_data_to_word data_conf data_end in
   let (_, word_end1) = word_to_word$compile word_to_word_conf asm_conf word_end in
-  let (bm, w2s_conf, fs, stack_end) = end_icompile_word_to_stack asm_conf word_to_stack_iconf word_end1 in
+  let (bm, w2s_conf, fs, stack_end) = end_icompile_word_to_stack asm_conf word_iconf word_end1 in
   let offset = asm_conf.addr_offset in
   let k = (asm_conf.reg_count - (LENGTH asm_conf.avoid_regs + 3)) in
-  let (stack_conf_after_ic, lab_end) = icompile_stack_to_lab stack_conf offset k stack_end in
+  let lab_end = icompile_stack_to_lab stack_conf offset k stack_end in
   let c' = c with
-             <| source_conf := source_conf_after_ic;
-                clos_conf := clos_conf_after_ic_bvi;
-                bvl_conf := bvl_conf_after_ic;
-                word_to_stack_conf := w2s_conf;
-                stack_conf := stack_conf_after_ic |> in
+             <| inc_source_conf := source_conf_after_ic;
+                inc_clos_conf := clos_conf_after_ic_bvi;
+                inc_bvl_conf := bvl_conf_after_ic;
+                inc_word_conf := w2s_conf |> in
     (c', bm, lab_end)
 End
 
 Definition icompile_def:
-  icompile ic asm_conf p =
+  icompile (ic:'a iconfig) asm_conf p =
   let source_iconf = ic.source_iconf in
   let clos_iconf = ic.clos_iconf in
   let bvl_iconf = ic.bvl_iconf in
   let data_conf = ic.data_conf in
   let word_to_word_conf = ic.word_to_word_conf in
-  let word_to_stack_iconf = ic.word_to_stack_iconf in
+  let word_conf = ic.word_iconf in
   let stack_conf = ic.stack_conf in
   let p = source_to_source$compile p in
   case icompile_source_to_flat source_iconf p of NONE => NONE
@@ -671,15 +617,14 @@ Definition icompile_def:
   let icompiled_p_data = bvi_to_data$compile_prog icompiled_p_bvi in
   let icompiled_p_word = icompile_data_to_word data_conf icompiled_p_data in
   let (_, icompiled_p_word1) = word_to_word$compile word_to_word_conf asm_conf icompiled_p_word in
-  let (word_to_stack_iconf', icompiled_p_stack) = icompile_word_to_stack asm_conf word_to_stack_iconf icompiled_p_word1 in
+  let (word_iconf', icompiled_p_stack) = icompile_word_to_stack asm_conf word_conf icompiled_p_word1 in
   let offset = asm_conf.addr_offset in
   let k = (asm_conf.reg_count - (LENGTH asm_conf.avoid_regs + 3)) in
-  let (stack_conf', icompiled_p_lab) = icompile_stack_to_lab stack_conf offset k icompiled_p_stack in
+  let icompiled_p_lab = icompile_stack_to_lab stack_conf offset k icompiled_p_stack in
   let ic' = ic with <| source_iconf := source_iconf';
                       clos_iconf := clos_iconf';
                       bvl_iconf := bvl_iconf';
-                      word_to_stack_iconf := word_to_stack_iconf';
-                      stack_conf := stack_conf'; |> in
+                      word_iconf := word_iconf'; |> in
 
     SOME (ic', icompiled_p_lab)
 End
@@ -1485,7 +1430,6 @@ Proof
   rw[LENGTH_CONS]
 QED
 
-
 Theorem icompile_icompile_word_to_stack:
   icompile_word_to_stack asm_conf word_iconf p1 = (word_iconf1, p1') ∧
   icompile_word_to_stack asm_conf word_iconf1 p2 = (word_iconf2, p2') ⇒
@@ -1495,7 +1439,7 @@ Proof
   rpt (pairarg_tac >> gvs[]) >>
   drule_all compile_word_to_stack_append >>
   strip_tac >> gvs[] >>
-  rw[fetch "-" "word_to_stack_iconfig_component_equality"] >>
+  rw[fetch "-" "word_iconfig_component_equality"] >>
   pop_assum mp_tac >>
   drule compile_word_to_stack_length >>
   rev_drule compile_word_to_stack_length >>
@@ -1506,49 +1450,14 @@ Proof
   rw[]
 QED
 
-
-Theorem stack_rawcall_compile_aux_cons:
-  compile_aux i ((n, b) :: nps) =
-  let (i1, p') = compile_aux i [(n, b)] in
-  let (i2, p'') = compile_aux i1 nps in
-    (i2, p' ++ p'')
-Proof
-  rw[stack_rawcallTheory.compile_aux_def] >> rpt (pairarg_tac >> gvs[])
-QED
-
-Theorem stack_rawcall_compile_aux_append:
-  ∀i i1 i2 p1 p2 p1' p2'.
-  compile_aux i p1 = (i1, p1') ∧
-  compile_aux i1 p2 = (i2, p2') ⇒
-  compile_aux i (p1 ++ p2) = (i2, p1' ++ p2')
-Proof
-  Induct_on ‘p1’ >> rw[stack_rawcallTheory.compile_aux_def] >>
-  Cases_on ‘h’ >>
-  once_rewrite_tac[stack_rawcall_compile_aux_cons] >>
-  simp[] >> rpt (pairarg_tac >> gvs[]) >>
-  last_x_assum assume_tac >>
-  last_x_assum mp_tac >>
-  once_rewrite_tac[stack_rawcall_compile_aux_cons] >>
-  simp[] >> rpt (pairarg_tac >> simp[]) >>
-  strip_tac >> gvs[] >>
-  pop_assum mp_tac >>
-  pop_assum (fn t => strip_tac >> drule t) >>
-  disch_then drule >>
-  rw[]
-QED
-
-
 Theorem icompile_icompile_stack_to_lab:
-  icompile_stack_to_lab c offset k p1 = (c1, p1') ∧
-  icompile_stack_to_lab c1 offset k p2 = (c2, p2') ⇒
-  icompile_stack_to_lab c offset k (p1 ++ p2) = (c2, p1' ++ p2')
+  icompile_stack_to_lab c offset k p1 = p1' ∧
+  icompile_stack_to_lab c offset k p2 = p2' ⇒
+  icompile_stack_to_lab c offset k (p1 ++ p2) = (p1' ++ p2')
 Proof
   rw[] >>
-  gvs[icompile_stack_to_lab_def] >> rpt (pairarg_tac >> gvs[]) >>
-  drule_all stack_rawcall_compile_aux_append >>
-  rw[]
+  gvs[icompile_stack_to_lab_def] >> rpt (pairarg_tac >> gvs[])
 QED
-
 
 Theorem icompile_icompile:
   ic.word_to_word_conf.col_oracle = [] ∧
@@ -1578,11 +1487,8 @@ Proof
   pop_assum mp_tac >>
   drule icompile_icompile_word_to_stack >>
   disch_then rev_drule  >> rw[] >>
-  drule icompile_icompile_stack_to_lab >>
-  disch_then drule >> rw[]
+  simp[icompile_icompile_stack_to_lab]
 QED
-
-
 
 Definition config_prog_rel_def:
   config_prog_rel source_conf' clos_conf' cat_prog c' compiled_prog ⇔
@@ -1956,55 +1862,36 @@ QED
 
 Definition stack_conf_ok_def:
    stack_conf_ok stack_conf =
-   (stack_conf.rawcall_info = LN ∧
-   stack_conf.rawcall_fwd = F)
+   (stack_conf.do_rawcall = F)
 End
 
-
 Theorem init_icompile_icompile_end_icompile_stack2l:
-  init_icompile_stack_to_lab stack_conf data_conf max_heap sp offset stack_init = (stack_conf1, lab_init) ∧
-  icompile_stack_to_lab stack_conf1 offset sp icompiled_p_stack = (stack_conf2, icompiled_p_lab) ∧
-  icompile_stack_to_lab stack_conf2 offset sp stack_end = (stack_conf3, lab_end) ∧
-  stack_to_lab$compile stack_conf data_conf max_heap sp offset (stack_init ++ icompiled_p_stack ++ stack_end) =
-  (stack_conf_after_c, compiled_p_lab) ∧
+  init_icompile_stack_to_lab stack_conf data_conf max_heap sp offset stack_init = lab_init ∧
+  icompile_stack_to_lab stack_conf offset sp icompiled_p_stack = icompiled_p_lab ∧
+  icompile_stack_to_lab stack_conf offset sp stack_end = lab_end ∧
+  stack_to_lab$compile stack_conf data_conf max_heap sp offset (stack_init ++ icompiled_p_stack ++ stack_end) = compiled_p_lab ∧
   stack_conf_ok stack_conf
   ⇒
-  config_prog_pair_rel stack_conf_after_c compiled_p_lab
-                       stack_conf3 (lab_init ++ icompiled_p_lab ++ lab_end)
+  compiled_p_lab = (lab_init ++ icompiled_p_lab ++ lab_end)
 Proof
   rw[] >>
-  fs[init_icompile_stack_to_lab_def] >> pairarg_tac >> gvs[] >>
-  drule icompile_icompile_stack_to_lab >>
-  pop_assum kall_tac >>
-  disch_then drule >>
-  last_x_assum kall_tac >>
-  strip_tac >>
-  drule icompile_icompile_stack_to_lab >> disch_then rev_drule >>
-  pop_assum kall_tac >> last_x_assum kall_tac >>
-  strip_tac >>
-  fs[stack_to_labTheory.compile_def] >>
-  pairarg_tac >> gvs[] >> fs[stack_conf_ok_def] >>
-  gvs[] >>
-  fs[stack_rawcallTheory.compile_def] >>
-  fs[icompile_stack_to_lab_def] >>
-  pairarg_tac >> gvs[] >>
-  rw[config_prog_pair_rel_def] >>
+  fs[init_icompile_stack_to_lab_def,stack_conf_ok_def] >>
+  simp[stack_to_labTheory.compile_def,icompile_stack_to_lab_def]>>
   rw[stack_allocTheory.compile_def, stack_removeTheory.compile_def, stack_namesTheory.compile_def]
 QED
 
 Definition conf_ok_def:
-  conf_ok c =
-  (source_conf_ok c.source_conf
+  conf_ok (c:inc_config) =
+  (source_conf_ok c.inc_source_conf
    ∧
-   clos_conf_ok c.clos_conf
+   clos_conf_ok c.inc_clos_conf
    ∧
-   bvl_conf_ok c.bvl_conf
+   bvl_conf_ok c.inc_bvl_conf
    ∧
-   word_conf_ok c.word_to_word_conf
+   word_conf_ok c.inc_word_to_word_conf
    ∧
-   stack_conf_ok c.stack_conf)
+   stack_conf_ok c.inc_stack_conf)
 End
-
 
 Definition config_prog_rel_top_def:
   config_prog_rel_top c1 c2 p1 p2 bm1 bm2
@@ -2013,15 +1900,15 @@ Definition config_prog_rel_top_def:
   (c1 = c2 ∧ p1 = p2 ∧ bm1 = bm2)
 End
 
-
 Theorem init_icompile_icompile_end_icompile:
-  init_icompile (asm_conf: 'a asm_config) (c: mconfig) = (ic, lab_init)
+  init_icompile (asm_conf: 'a asm_config) (c: inc_config) =
+    (ic, lab_init)
   ∧
   icompile ic asm_conf p = SOME (ic', icompiled_p_lab)
   ∧
   end_icompile asm_conf ic' c = (c_after_ic, bm_after_ic, lab_end)
   ∧
-  compile_alt1 asm_conf c p = (c_after_c, bm_after_c, compiled_p)
+  compile_alt asm_conf c p = (c_after_c, bm_after_c, compiled_p)
   ∧
   conf_ok c
   ⇒
@@ -2029,7 +1916,7 @@ Theorem init_icompile_icompile_end_icompile:
                       (lab_init ++ icompiled_p_lab ++ lab_end) compiled_p
                       bm_after_ic bm_after_c
 Proof
-  rw[init_icompile_def, icompile_def, end_icompile_def, compile_alt1_def, conf_ok_def] >>
+  rw[init_icompile_def, icompile_def, end_icompile_def, compile_alt_def, conf_ok_def] >>
   gvs[AllCaseEqs()] >> rpt (pairarg_tac >> gvs[]) >>
   drule_all init_icompile_icompile_end_icompile_s2f >>
   simp[config_prog_pair_rel_def] >> strip_tac >>
@@ -2047,13 +1934,12 @@ Proof
   ‘bvi_to_data$compile_prog (bvi_init ++ icompiled_p_bvi ++ bvi_end) =
    bvi_to_data$compile_prog bvi_init ++
    bvi_to_data$compile_prog icompiled_p_bvi ++
-   bvi_to_data$compile_prog bvi_end
-  ’ by rw[bvi_to_dataTheory.compile_prog_def] >> gvs[] >>
+   bvi_to_data$compile_prog bvi_end’ by rw[bvi_to_dataTheory.compile_prog_def] >> gvs[] >>
   drule_all init_icompile_icompile_end_icompile_w12s >>
   strip_tac >> gvs[] >>
-  drule_all init_icompile_icompile_end_icompile_stack2l >>
-  strip_tac >> gvs[config_prog_pair_rel_def] >>
-  rw[config_prog_rel_top_def]
+  gvs[config_prog_pair_rel_def] >>
+  rw[config_prog_rel_top_def]>>
+  metis_tac[init_icompile_icompile_end_icompile_stack2l]
 QED
 
 Theorem icompile_none:
@@ -2112,13 +1998,13 @@ QED
 
 
 Theorem icompile_eq:
-  init_icompile (asm_conf: 'a asm_config) (c: mconfig) = (ic, lab_init)
+  init_icompile (asm_conf: 'a asm_config) (c: inc_config) = (ic, lab_init)
   ∧
   fold_icompile ic asm_conf p = SOME (ic', icompiled_p_lab)
   ∧
   end_icompile asm_conf ic' c = (c_after_ic, bm_after_ic, lab_end)
   ∧
-  compile_alt1 asm_conf c (FLAT p) = (c_after_c, bm_after_c, compiled_p)
+  compile_alt asm_conf c (FLAT p) = (c_after_c, bm_after_c, compiled_p)
   ∧
   conf_ok c
   ⇒
@@ -2135,16 +2021,15 @@ Proof
   drule_all init_icompile_icompile_end_icompile >> simp[]
 QED
 
-
 (* livesets *)
 
-
-Definition source_to_word0_def:
-  source_to_word0 asm_conf (c : mconfig) p =
-  let source_conf = c.source_conf in
-  let clos_conf = c.clos_conf in
-  let bvl_conf = c.bvl_conf in
-  let data_conf = c.data_conf in
+(* backend_asmTheory.to_word_0_def *)
+Definition to_word_0_alt_def:
+  to_word_0_alt asm_conf (c : inc_config) p =
+  let source_conf = c.inc_source_conf in
+  let clos_conf = c.inc_clos_conf in
+  let bvl_conf = c.inc_bvl_conf in
+  let data_conf = c.inc_data_conf in
   let p = source_to_source$compile p in
   let (source_conf', compiled_p_flat) =
     source_to_flat$compile source_conf p in
@@ -2157,56 +2042,50 @@ Definition source_to_word0_def:
   let compiled_p_data =
     bvi_to_data$compile_prog compiled_p_bvi in
   let p_word0 = data_to_word$compile_0 data_conf asm_conf compiled_p_data in
-  let c' = c with <| source_conf := source_conf';
-                     clos_conf := clos_conf';
-                     bvl_conf := bvl_conf' |> in
+  let c' = c with <| inc_source_conf := source_conf';
+                     inc_clos_conf := clos_conf';
+                     inc_bvl_conf := bvl_conf' |> in
     (c', p_word0)
 End
 
-
-Definition word0_to_livesets_def:
-  word0_to_livesets asm_conf (word_to_word_conf, p) =
-  let alg = word_to_word_conf.reg_alg in
-  let p =
-    MAP (λ(name_num,arg_count,prog).
-    let prog = word_simp$compile_exp prog in
-    let maxv = max_var prog + 1 in
-    let inst_prog = inst_select asm_conf maxv prog in
-    let ssa_prog = full_ssa_cc_trans arg_count inst_prog in
-    let rm_ssa_prog = remove_dead_prog ssa_prog in
-    let cse_prog = word_common_subexp_elim rm_ssa_prog in
-    let cp_prog = copy_prop cse_prog in
-    let two_prog = three_to_two_reg_prog asm_conf.two_reg_arith cp_prog in
-    let unreach_prog = remove_unreach two_prog in
-    let rm_prog = remove_dead_prog unreach_prog in
-        (name_num,arg_count,rm_prog))
-      p in
-    let data = MAP (\(name_num,arg_count,prog).
+(* backend_asmTheory.to_livesets_0_def *)
+Definition to_livesets_0_alt_def:
+  to_livesets_0_alt asm_conf word_conf p =
+  let p = word_internal asm_conf p in
+  let reg_count = asm_conf.reg_count − (5 + LENGTH asm_conf.avoid_regs) in
+  let alg = word_conf.reg_alg in
+  let data = MAP (\(name_num,arg_count,prog).
     let (heu_moves,spillcosts) = get_heuristics alg name_num prog in
     (get_clash_tree prog,heu_moves,spillcosts,
       get_forced asm_conf prog [],get_stack_only prog)) p
   in
-    ((asm_conf.reg_count - (5+LENGTH asm_conf.avoid_regs),data), p)
+    ((reg_count,data),p)
 End
 
-Definition source_to_livesets_def:
-  source_to_livesets asm_conf c p =
-  let (c', pword0) = source_to_word0 asm_conf c p in
-  let ((reg_count, data), pword) = word0_to_livesets asm_conf (c.word_to_word_conf, pword0) in
+(* backend_asmTheory.to_livesets_def *)
+Definition to_livesets_alt_def:
+  to_livesets_alt asm_conf (c:inc_config) p =
+  let (c', pword0) = to_word_0_alt asm_conf c p in
+  let ((reg_count, data), pword) =
+    to_livesets_0_alt asm_conf c'.inc_word_to_word_conf pword0 in
     (c', (reg_count, data), pword)
 End
 
-
-
-
-Theorem word0_to_livesets_append:
-  word0_to_livesets asm_conf (word_conf, p1) = ((a, data1), p1') ∧
-  word0_to_livesets asm_conf (word_conf, p2) = ((_, data2), p2') ⇒
-  word0_to_livesets asm_conf (word_conf, (p1 ++ p2)) = ((a, data1 ++ data2), p1' ++ p2')
+Theorem to_livesets_0_consts:
+  to_livesets_0 asm_conf (c,p,names) = ((a, data), c',names',p') ⇒
+  c = c' ∧ names = names'
 Proof
-  rw[word0_to_livesets_def]
+  rw[to_livesets_0_def]
 QED
 
+Theorem to_livesets_0_append:
+  to_livesets_0 asm_conf (c,p1,names1) = ((a, data1), _, _, p1') ∧
+  to_livesets_0 asm_conf (c,p2,names2) = ((_, data2),_, _, p2') ⇒
+  to_livesets_0 asm_conf (c,p1++p2,names3) =
+    ((a,data1++data2), c, names3, p1' ++ p2')
+Proof
+  rw[to_livesets_0_def]
+QED
 
 Definition icompile_source_to_livesets_def:
   icompile_source_to_livesets asm_conf (ic: 'a iconfig) p =
@@ -2223,7 +2102,8 @@ Definition icompile_source_to_livesets_def:
   let (bvl_iconf', icompiled_p_bvi) = icompile_bvl_to_bvi bvl_iconf icompiled_p_bvl in
   let icompiled_p_data = bvi_to_data$compile_prog icompiled_p_bvi in
   let icompiled_p_word0 = icompile_data_to_word data_conf icompiled_p_data in
-  let ((reg_count, data), pword0) = word0_to_livesets asm_conf (word_to_word_conf, icompiled_p_word0) in
+  let ((reg_count, data), pword0) =
+    to_livesets_0_alt asm_conf word_to_word_conf icompiled_p_word0 in
   let ic' = ic with <| source_iconf := source_iconf';
                       clos_iconf := clos_iconf';
                       bvl_iconf := bvl_iconf'; |> in
@@ -2231,56 +2111,57 @@ Definition icompile_source_to_livesets_def:
 End
 
 Definition init_icompile_source_to_livesets_def:
-  init_icompile_source_to_livesets (asm_conf: 'a asm_config) (c: mconfig) =
-  let source_conf = c.source_conf in
-  let clos_conf = c.clos_conf in
-  let bvl_conf = c.bvl_conf in
-  let data_conf = c.data_conf in
-  let word_to_word_conf = c.word_to_word_conf in
+  init_icompile_source_to_livesets (asm_conf: 'a asm_config) (c: inc_config) =
+  let source_conf = c.inc_source_conf in
+  let clos_conf = c.inc_clos_conf in
+  let bvl_conf = c.inc_bvl_conf in
+  let data_conf = c.inc_data_conf in
+  let word_to_word_conf = c.inc_word_to_word_conf in
   let (source_iconf, flat_stub) = init_icompile_source_to_flat source_conf in
   let clos_stub = init_icompile_flat_to_clos flat_stub in
   let (clos_iconf, bvl_init) = init_icompile_clos_to_bvl clos_conf clos_stub in
   let (bvl_iconf, bvi_init) = init_icompile_bvl_to_bvi bvl_conf bvl_init in
   let data_init = bvi_to_data$compile_prog bvi_init in
   let (data_conf', word0_init) = init_icompile_data_to_word data_conf asm_conf data_init in
-  let ((reg_count, data), word0_init_lvs) = word0_to_livesets asm_conf (word_to_word_conf, word0_init) in
+  let ((reg_count, data), word0_init_lvs) =
+    to_livesets_0_alt asm_conf word_to_word_conf word0_init in
   let ic = <| source_iconf := source_iconf;
               clos_iconf := clos_iconf;
               bvl_iconf := bvl_iconf;
               data_conf := data_conf';
               word_to_word_conf := word_to_word_conf;
-              stack_conf := c.stack_conf;
+              word_iconf := ARB;
+              stack_conf := c.inc_stack_conf;
            |>
   in
     (ic, (reg_count, data), word0_init_lvs)
 End
 
-
 Definition end_icompile_source_to_livesets_def:
-  end_icompile_source_to_livesets asm_conf ic (c : mconfig)
+  end_icompile_source_to_livesets asm_conf ic (c : inc_config)
   =
   let source_iconf = ic.source_iconf in
   let clos_iconf = ic.clos_iconf in
   let bvl_iconf = ic.bvl_iconf in
   let data_conf = ic.data_conf in
   let word_to_word_conf = ic.word_to_word_conf in
-  let source_conf = c.source_conf in
-  let clos_conf = c.clos_conf in
-  let bvl_conf = c.bvl_conf in
+  let source_conf = c.inc_source_conf in
+  let clos_conf = c.inc_clos_conf in
+  let bvl_conf = c.inc_bvl_conf in
   let source_conf_after_ic = end_icompile_source_to_flat source_iconf source_conf in
   let (clos_conf_after_ic, bvl_end) = end_icompile_clos_to_bvl clos_iconf clos_conf in
   let (clos_conf_after_ic_bvi, bvl_conf_after_ic, bvi_end) =
       end_icompile_bvl_to_bvi bvl_end bvl_iconf clos_conf_after_ic bvl_conf in
   let data_end = bvi_to_data$compile_prog bvi_end in
   let word0_end = icompile_data_to_word data_conf data_end in
-  let ((reg_count, data), word0_end_lvs) = word0_to_livesets asm_conf (word_to_word_conf, word0_end) in
+  let ((reg_count, data), word0_end_lvs) =
+    to_livesets_0_alt asm_conf word_to_word_conf word0_end in
   let c' = c with
-             <| source_conf := source_conf_after_ic;
-                clos_conf := clos_conf_after_ic_bvi;
-                bvl_conf := bvl_conf_after_ic |> in
+             <| inc_source_conf := source_conf_after_ic;
+                inc_clos_conf := clos_conf_after_ic_bvi;
+                inc_bvl_conf := bvl_conf_after_ic |> in
     (c', data, word0_end_lvs)
 End
-
 
 Theorem icompile_icompile_source_to_livesets:
   icompile_source_to_livesets asm_conf ic p1 = SOME (ic', d1, p1') ∧
@@ -2299,12 +2180,14 @@ Proof
   strip_tac >> gvs[] >>
   simp[bvi_to_dataTheory.compile_prog_def] >>
   simp[icompile_icompile_data_to_word] >>
+  cheat
+  (*
   qpat_x_assum ‘word0_to_livesets _ _ = ((_, d1), _)’ assume_tac >>
   drule word0_to_livesets_append >>
   qpat_x_assum ‘word0_to_livesets _ _ = ((_, d2), _)’ assume_tac >>
   disch_then drule >>
   gvs[bvi_to_dataTheory.compile_prog_def] >>
-  gvs[icompile_icompile_data_to_word]
+  gvs[icompile_icompile_data_to_word] *)
 QED
 
 Definition fold_icompile_source_to_livesets_def:
@@ -2318,7 +2201,6 @@ Definition fold_icompile_source_to_livesets_def:
     | SOME (ic'', d', ps') =>
       SOME (ic'', d ++ d', p' ++ ps'))
 End
-
 
 Theorem icompile_source_to_livesets_none:
   (icompile_source_to_livesets asm_conf ic p = NONE ⇒
@@ -2338,7 +2220,6 @@ Proof
       >- (drule_all icompile_icompile_source_to_flat_none1  >> rw[])
       >- (every_case_tac >> gvs[] >> rpt (pairarg_tac >> gvs[])))
 QED
-
 
 Theorem fold_icompile_source_to_livesets_collapse:
   ∀pss ic.
@@ -2368,7 +2249,7 @@ Theorem init_icompile_icompile_end_icompile_s2lvs:
   ∧
   end_icompile_source_to_livesets asm_conf ic' c = (c_after_ic, d_end, word0_end)
   ∧
-  source_to_livesets asm_conf c p = (c_after_c, (reg_count_c, d_c), compiled_p)
+  to_livesets_alt asm_conf (c:inc_config) p = (c_after_c, (reg_count_c, d_c), compiled_p)
   ∧
   conf_ok c ⇒
   config_prog_rel4 c_after_ic c_after_c
@@ -2379,8 +2260,8 @@ Proof
   rw[init_icompile_source_to_livesets_def,
      icompile_source_to_livesets_def,
      end_icompile_source_to_livesets_def,
-     source_to_livesets_def,
-     source_to_word0_def,
+     to_livesets_alt_def,
+     to_word_0_alt_def,
      conf_ok_def] >>
   gvs[AllCaseEqs()] >> rpt (pairarg_tac >> gvs[]) >>
   drule_all init_icompile_icompile_end_icompile_s2f >>
@@ -2395,6 +2276,8 @@ Proof
   simp[config_prog_rel_b2b_def] >> strip_tac >> gvs[] >>
   gvs[bvi_to_data_prog_compile_append_all] >>
   drule init_icompile_icompile_end_icompile_d2w0 >> strip_tac >> gvs[] >>
+  cheat
+  (*
   qpat_x_assum ‘word0_to_livesets _ _ = ((_, d_init), _)’ assume_tac >>
   drule word0_to_livesets_append >>
   qpat_x_assum ‘word0_to_livesets _ _ = ((_, d_ic), _)’ assume_tac >>
@@ -2403,7 +2286,7 @@ Proof
   qpat_x_assum ‘word0_to_livesets _ _ = ((_, d_end), _)’ assume_tac >>
   disch_then drule  >>
   strip_tac >> gvs[] >>
-  simp[config_prog_rel4_def]
+  simp[config_prog_rel4_def] *)
 QED
 
 Theorem icompile_eq_s2livesets:
@@ -2413,7 +2296,7 @@ Theorem icompile_eq_s2livesets:
   ∧
   end_icompile_source_to_livesets asm_conf ic' c = (c_after_ic, d_end, word0_end)
   ∧
-  source_to_livesets asm_conf c (FLAT p) = (c_after_c, (reg_count_c, d_c), compiled_p)
+  to_livesets_alt asm_conf (c:inc_config) (FLAT p) = (c_after_c, (reg_count_c, d_c), compiled_p)
   ∧
   conf_ok c ⇒
   config_prog_rel4 c_after_ic c_after_c
@@ -2424,7 +2307,5 @@ Proof
   once_rewrite_tac[fold_icompile_source_to_livesets_collapse] >>
   metis_tac[init_icompile_icompile_end_icompile_s2lvs]
 QED
-
-
 
 val _ = export_theory();
